Make `parse_nondep_then_rtol` more general

src/lowparse/LowParse.Spec.RtoLPair.fst
@@ -18,16 +18,16 @@ let nondep_then_rtol_bare
   (#k1: parser_kind)
   (#t1: Type)
   (p1: parser k1 t1 { k1.parser_kind_subkind == Some ParserConsumesAll })
-  (#n: nat)
+  (#k2: parser_kind)
   (#t2: Type)
-  (p2: parser (total_constant_size_parser_kind n) t2)
+  (p2: parser k2 t2 { k2.parser_kind_high == Some (k2.parser_kind_low) } )
 : Tot (bare_parser (t2 & t1))
   =
   fun b ->
-    if Seq.length b < n then
+    if Seq.length b < k2.parser_kind_low then
       None
     else
-      let (bl, br) = Seq.split b (Seq.length b - n) in
+      let (bl, br) = Seq.split b (Seq.length b - k2.parser_kind_low) in
       match parse p2 br with
       | Some (x2, consumed2) ->
         begin match parse p1 bl with
@@ -41,16 +41,16 @@ let nondep_then_rtol_bare_correct
   (#k1: parser_kind)
   (#t1: Type)
   (p1: parser k1 t1 { k1.parser_kind_subkind == Some ParserConsumesAll })
-  (#n: nat)
+  (#k2: parser_kind)
   (#t2: Type)
-  (p2: parser (total_constant_size_parser_kind n) t2)
-  : Lemma (ensures parser_kind_prop (nondep_then_rtol_kind k1 n) (nondep_then_rtol_bare
+  (p2: parser k2 t2 { k2.parser_kind_high == Some (k2.parser_kind_low) } )
+  : Lemma (ensures parser_kind_prop (nondep_then_rtol_kind k1 k2.parser_kind_low) (nondep_then_rtol_bare
     p1 p2))
   = 
     Classical.forall_intro_2 (Seq.lemma_split # byte) ;
     parser_kind_prop_equiv k1 p1;
-    parser_kind_prop_equiv (total_constant_size_parser_kind n) p2;
-    parser_kind_prop_equiv (nondep_then_rtol_kind k1 n) (nondep_then_rtol_bare
+    parser_kind_prop_equiv k2 p2;
+    parser_kind_prop_equiv (nondep_then_rtol_kind k1 k2.parser_kind_low) (nondep_then_rtol_bare
     p1 p2);
 
     let ps = nondep_then_rtol_bare p1 p2 in
@@ -60,8 +60,8 @@ let nondep_then_rtol_bare_correct
       (requires (injective_precond ps b1 b2))
       (ensures (injective_postcond ps b1 b2))
     = 
-      let (bl1, br1) = Seq.split b1 (Seq.length b1 - n) in
-      let (bl2, br2) = Seq.split b2 (Seq.length b2 - n) in
+      let (bl1, br1) = Seq.split b1 (Seq.length b1 - k2.parser_kind_low) in
+      let (bl2, br2) = Seq.split b2 (Seq.length b2 - k2.parser_kind_low) in
       assert (injective_precond p2 br1 br2);
       assert (injective_precond p1 bl1 bl2);
       assert (injective_postcond ps b1 b2)
@@ -69,26 +69,26 @@ let nondep_then_rtol_bare_correct
     Classical.forall_intro_2 (fun x -> Classical.move_requires (f x)) ; // add f to the SMT context
     assert (injective (nondep_then_rtol_bare p1 p2));
     assert (consumes_all (nondep_then_rtol_bare p1 p2));
-    assert (parses_at_least (k1.parser_kind_low + n) (nondep_then_rtol_bare p1 p2))
+    assert (parses_at_least (k1.parser_kind_low + k2.parser_kind_low) (nondep_then_rtol_bare p1 p2))
 
 
 val parse_nondep_then_rtol
   (#k1: parser_kind)
   (#t1: Type)
   (p1: parser k1 t1 { k1.parser_kind_subkind == Some ParserConsumesAll })
-  (#n: nat)
+  (#k2: parser_kind)
   (#t2: Type)
-  (p2: parser (total_constant_size_parser_kind n) t2)
-: Tot (parser (nondep_then_rtol_kind k1 n) (t2 & t1))
+  (p2: parser k2 t2 { k2.parser_kind_high == Some (k2.parser_kind_low) } )
+: Tot (parser (nondep_then_rtol_kind k1 k2.parser_kind_low) (t2 & t1))
 
 let parse_nondep_then_rtol
   (#k1: parser_kind)
   (#t1: Type)
   (p1: parser k1 t1 { k1.parser_kind_subkind == Some ParserConsumesAll })
-  (#n: nat)
+  (#k2: parser_kind)
   (#t2: Type)
-  (p2: parser (total_constant_size_parser_kind n) t2)
-  : Tot (parser (nondep_then_rtol_kind k1 n) (t2 & t1)) =
+  (p2: parser k2 t2 { k2.parser_kind_high == Some (k2.parser_kind_low) } )
+  : Tot (parser (nondep_then_rtol_kind k1 k2.parser_kind_low) (t2 & t1)) =
   nondep_then_rtol_bare_correct p1 p2;
   nondep_then_rtol_bare p1 p2
 
